smallstep.v

Smallstep.v
@@ -8,7 +8,7 @@ Require Export Imp.
     "big-step" style -- they specify how a given expression can be
     evaluated to its final value (or a command plus a store to a final
     store) "all in one big step."
- 
+
     This style is simple and natural for many purposes -- indeed,
     Gilles Kahn, who popularized its use, called it _natural
     semantics_.  But there are some things it does not do well.  In
@@ -49,7 +49,7 @@ Require Export Imp.
     the program tries to do an operation that makes no sense, such as
     adding a number to a list, and none of the evaluation rules can be
     applied.
- 
+
     These two outcomes -- nontermination vs. getting stuck in an
     erroneous configuration -- are quite different.  In particular, we
     want to allow the first (permitting the possibility of infinite
@@ -60,7 +60,7 @@ Require Export Imp.
     topic for the rest of the course.  As a first step, we need a
     different way of presenting the semantics that allows us to
     distinguish nontermination from erroneous "stuck states."
- 
+
     So, for lots of reasons, we'd like to have a finer-grained way of
     defining and reasoning about program behaviors.  This is the topic
     of the present chapter.  We replace the "big-step" [eval] relation
@@ -97,7 +97,7 @@ Fixpoint evalF (t : tm) : nat :=
 (** Now, here is the same evaluator, written in exactly the same
     style, but formulated as an inductively defined relation.  Again,
     we use the notation [t || n] for "[t] evaluates to [n]." *)
-(** 
+(**
                                --------                                (E_Const)
                                C n || n
 
@@ -107,13 +107,13 @@ Fixpoint evalF (t : tm) : nat :=
                         P t1 t2 || C (n1 + n2)
 *)
 
-Reserved Notation " t '||' n " (at level 50, left associativity). 
+Reserved Notation " t '||' n " (at level 50, left associativity).
 
 Inductive eval : tm -> nat -> Prop :=
   | E_Const : forall n,
       C n || n
-  | E_Plus : forall t1 t2 n1 n2, 
-      t1 || n1 -> 
+  | E_Plus : forall t1 t2 n1 n2,
+      t1 || n1 ->
       t2 || n2 ->
       P t1 t2 || (n1 + n2)
 
@@ -126,7 +126,7 @@ Tactic Notation "eval_cases" tactic(first) ident(c) :=
 Module SimpleArith1.
 
 (** Now, here is a small-step version. *)
-(** 
+(**
                      -------------------------------        (ST_PlusConstConst)
                      P (C n1) (C n2) ==> C (n1 + n2)
 
@@ -150,7 +150,7 @@ Inductive step : tm -> tm -> Prop :=
       t1 ==> t1' ->
       P t1 t2 ==> P t1' t2
   | ST_Plus2 : forall n1 t2 t2',
-      t2 ==> t2' -> 
+      t2 ==> t2' ->
       P (C n1) t2 ==> P (C n1) t2'
 
   where " t '==>' t' " := (step t t').
@@ -161,7 +161,7 @@ Tactic Notation "step_cases" tactic(first) ident(c) :=
   | Case_aux c "ST_Plus1" | Case_aux c "ST_Plus2" ].
 
 (** Things to notice:
- 
+
     - We are defining just a single reduction step, in which
       one [P] node is replaced by its value.
 
@@ -179,12 +179,12 @@ Tactic Notation "step_cases" tactic(first) ident(c) :=
 (** If [t1] can take a step to [t1'], then [P t1 t2] steps
     to [P t1' t2]: *)
 
-Example test_step_1 : 
-      P 
+Example test_step_1 :
+      P
         (P (C 0) (C 3))
         (P (C 2) (C 4))
       ==>
-      P 
+      P
         (C (0 + 3))
         (P (C 2) (C 4)).
 Proof.
@@ -196,20 +196,20 @@ Proof.
     then [P (C n) t2] steps to [P (C n)
     t2']: *)
 
-Example test_step_2 : 
-      P 
+Example test_step_2 :
+      P
         (C 0)
-        (P 
-          (C 2) 
+        (P
+          (C 2)
           (P (C 0) (C 3)))
       ==>
-      P 
+      P
         (C 0)
-        (P 
-          (C 2) 
+        (P
+          (C 2)
           (C (0 + 3))).
-Proof. 
-  (* FILL IN HERE *) Admitted.
+Proof.
+  repeat constructor. Qed.
 (** [] *)
 
 
@@ -256,7 +256,7 @@ Definition relation (X: Type) := X->X->Prop.
       - If both are [ST_PlusConstConst], the result is immediate.
 
       - The cases when both derivations end with [ST_Plus1] or
-        [ST_Plus2] follow by the induction hypothesis.  
+        [ST_Plus2] follow by the induction hypothesis.
 
       - It cannot happen that one is [ST_PlusConstConst] and the other
         is [ST_Plus1] or [ST_Plus2], since this would imply that [x] has
@@ -270,7 +270,7 @@ Definition relation (X: Type) := X->X->Prop.
         the form [C n]. [] *)
 
 Definition deterministic {X: Type} (R: relation X) :=
-  forall x y1 y2 : X, R x y1 -> R x y2 -> y1 = y2. 
+  forall x y1 y2 : X, R x y1 -> R x y2 -> y1 = y2.
 
 Theorem step_deterministic:
   deterministic step.
@@ -293,12 +293,12 @@ Proof.
       SCase "ST_Plus1". inversion H2.
       SCase "ST_Plus2".
         rewrite <- (IHHy1 t2'0).
-        reflexivity. assumption.  
+        reflexivity. assumption.
 Qed.
 
 (** There is some annoying repetition in this proof.
-    Each use of [inversion Hy2] results in three subcases, 
-    only one of which is relevant (the one which matches the 
+    Each use of [inversion Hy2] results in three subcases,
+    only one of which is relevant (the one which matches the
     current case in the induction on [Hy1]). The other two
     subcases need to be dismissed by finding the contradiction
     among the hypotheses and doing inversion on it.
@@ -317,10 +317,10 @@ Theorem step_deterministic_alt: deterministic step.
 Proof.
   intros x y1 y2 Hy1 Hy2.
   generalize dependent y2.
-  step_cases (induction Hy1) Case; intros y2 Hy2; 
+  step_cases (induction Hy1) Case; intros y2 Hy2;
     inversion Hy2; subst; try (solve by inversion).
   Case "ST_PlusConstConst". reflexivity.
-  Case "ST_Plus1". 
+  Case "ST_Plus1".
     apply IHHy1 in H2. rewrite H2. reflexivity.
   Case "ST_Plus2".
     apply IHHy1 in H2. rewrite H2. reflexivity.
@@ -369,7 +369,7 @@ Inductive value : tm -> Prop :=
     definition of the [==>] relation to write [ST_Plus2] rule in a
     slightly more elegant way: *)
 
-(** 
+(**
                      -------------------------------        (ST_PlusConstConst)
                      P (C n1) (C n2) ==> C (n1 + n2)
 
@@ -402,7 +402,7 @@ Inductive step : tm -> tm -> Prop :=
         t1 ==> t1' ->
         P t1 t2 ==> P t1' t2
   | ST_Plus2 : forall v1 t2 t2',
-        value v1 ->                     (* <----- n.b. *) 
+        value v1 ->                     (* <----- n.b. *)
         t2 ==> t2' ->
         P v1 t2 ==> P v1 t2'
 
@@ -414,7 +414,7 @@ Tactic Notation "step_cases" tactic(first) ident(c) :=
   | Case_aux c "ST_Plus1" | Case_aux c "ST_Plus2" ].
 
 (** **** Exercise: 3 stars (redo_determinism)  *)
-(** As a sanity check on this change, let's re-verify determinism 
+(** As a sanity check on this change, let's re-verify determinism
 
     Proof sketch: We must show that if [x] steps to both [y1] and [y2]
     then [y1] and [y2] are equal.  Consider the final rules used in
@@ -443,7 +443,22 @@ Tactic Notation "step_cases" tactic(first) ident(c) :=
 Theorem step_deterministic :
   deterministic step.
 Proof.
-  (* FILL IN HERE *) Admitted.
+  unfold deterministic. intros.
+  generalize dependent y2.
+  induction H; intros; inversion H0; subst; try (solve by inversion);
+  try reflexivity.
+  apply IHstep in H4; apply IHstep in H; subst; reflexivity.
+  inversion H3. subst. inversion H.
+  inversion H; subst.
+  inversion H1; subst; try (solve by inversion).
+  inversion H6; subst; try (solve by inversion). reflexivity.
+  inversion H; subst.
+  inversion H1; subst. inversion H6.
+  apply IHstep in H7. subst; reflexivity.
+  inversion H; subst.
+  inversion H1; subst. inversion H7.
+  apply IHstep in H8. rewrite H8. reflexivity.
+Qed.
 (** [] *)
 
 (* ########################################################### *)
@@ -478,7 +493,7 @@ Proof.
 
 Theorem strong_progress : forall t,
   value t \/ (exists t', t ==> t').
-Proof.  
+Proof.
   tm_cases (induction t) Case.
     Case "C". left. apply v_const.
     Case "P". right. inversion IHt1.
@@ -489,7 +504,7 @@ Proof.
         SSCase "r". inversion H0 as [t' H1].
           exists (P t1 t').
           apply ST_Plus2. apply H. apply H1.
-      SCase "r". inversion H as [t' H0]. 
+      SCase "r". inversion H as [t' H0].
           exists (P t' t2).
           apply ST_Plus1. apply H0.  Qed.
 
@@ -501,7 +516,7 @@ Proof.
 
 (** The idea of "making progress" can be extended to tell us something
     interesting about [value]s: in this language [value]s are exactly
-    the terms that _cannot_ make progress in this sense.  
+    the terms that _cannot_ make progress in this sense.
 
     To state this observation formally, let's begin by giving a name
     to terms that cannot make progress.  We'll call them _normal
@@ -543,28 +558,28 @@ Corollary nf_same_as_value : forall t,
 Proof.
   split. apply nf_is_value. apply value_is_nf. Qed.
 
-(** Why is this interesting?  
+(** Why is this interesting?
 
     Because [value] is a syntactic concept -- it is defined by looking
     at the form of a term -- while [normal_form] is a semantic one --
     it is defined by looking at how the term steps.  It is not obvious
     that these concepts should coincide!
- 
+
     Indeed, we could easily have written the definitions so that they
     would not coincide... *)
- 
+
 (* ##################################################### *)
 
 (** We might, for example, mistakenly define [value] so that it
     includes some terms that are not finished reducing. *)
 
-Module Temp1. 
+Module Temp1.
 (* Open an inner module so we can redefine value and step. *)
 
 Inductive value : tm -> Prop :=
 | v_const : forall n, value (C n)
 | v_funny : forall t1 n2,                       (* <---- *)
-              value (P t1 (C n2)).  
+              value (P t1 (C n2)).
 
 Reserved Notation " t '==>' t' " (at level 40).
 
@@ -587,7 +602,10 @@ Inductive step : tm -> tm -> Prop :=
 Lemma value_not_same_as_normal_form :
   exists v, value v /\ ~ normal_form step v.
 Proof.
-  (* FILL IN HERE *) Admitted.
+  unfold normal_form. unfold not. exists (P (C 1) (C 1)).
+  split. constructor.
+  intros. apply H. exists (C 2). constructor.
+Qed.
 (** [] *)
 End Temp1.
 
@@ -622,7 +640,10 @@ Inductive step : tm -> tm -> Prop :=
 Lemma value_not_same_as_normal_form :
   exists v, value v /\ ~ normal_form step v.
 Proof.
-  (* FILL IN HERE *) Admitted.
+  exists (C 1). split. constructor.
+  unfold normal_form. unfold not. intros. apply H.
+  exists (P (C 1) (C 0)). constructor.
+Qed.
 
 (** [] *)
 End Temp2.
@@ -657,7 +678,12 @@ Inductive step : tm -> tm -> Prop :=
 Lemma value_not_same_as_normal_form :
   exists t, ~ value t /\ normal_form step t.
 Proof.
-  (* FILL IN HERE *) Admitted.
+  exists (P (C 0) (P (C 0) (C 1))).
+  split. unfold not. intros. inversion H.
+  unfold normal_form; unfold not; intros.
+  destruct H. inversion H; subst.
+  inversion H3.
+Qed.
 (** [] *)
 
 End Temp3.
@@ -693,7 +719,7 @@ Inductive step : tm -> tm -> Prop :=
 
   where " t '==>' t' " := (step t t').
 
-(** **** Exercise: 1 star (smallstep_bools)  *) 
+(** **** Exercise: 1 star (smallstep_bools)  *)
 (** Which of the following propositions are provable?  (This is just a
     thought exercise, but for an extra challenge feel free to prove
     your answers in Coq.) *)
@@ -701,30 +727,30 @@ Inductive step : tm -> tm -> Prop :=
 Definition bool_step_prop1 :=
   tfalse ==> tfalse.
 
-(* FILL IN HERE *)
+(* no *)
 
 Definition bool_step_prop2 :=
      tif
        ttrue
        (tif ttrue ttrue ttrue)
        (tif tfalse tfalse tfalse)
-  ==> 
+  ==>
      ttrue.
 
-(* FILL IN HERE *)
+(* yes *)
 
 Definition bool_step_prop3 :=
      tif
        (tif ttrue ttrue ttrue)
        (tif ttrue ttrue ttrue)
        tfalse
-   ==> 
+   ==>
      tif
        ttrue
        (tif ttrue ttrue ttrue)
        tfalse.
 
-(* FILL IN HERE *)
+(* yes *)
 (** [] *)
 
 (** **** Exercise: 3 stars, optional (progress_bool)  *)
@@ -733,32 +759,46 @@ Definition bool_step_prop3 :=
 
 Theorem strong_progress : forall t,
   value t \/ (exists t', t ==> t').
-Proof.  
-  (* FILL IN HERE *) Admitted.
+Proof.
+  intros.
+  induction t;
+  try (left; constructor).
+  right. destruct IHt1.
+  inversion H; subst.
+  exists t2. constructor.
+  exists t3. constructor.
+  destruct H.
+  exists (tif x t2 t3). constructor. assumption.
+Qed.
 (** [] *)
 
 (** **** Exercise: 2 stars, optional (step_deterministic)  *)
 Theorem step_deterministic :
   deterministic step.
 Proof.
-  (* FILL IN HERE *) Admitted.
+  unfold deterministic. intros.
+  generalize dependent y2.
+  induction H; intros; inversion H0; subst;
+  try (solve by inversion); try reflexivity.
+  apply IHstep in H5; subst. reflexivity.
+Qed.
 (** [] *)
 
-Module Temp5. 
+Module Temp5.
 
-(** **** Exercise: 2 stars (smallstep_bool_shortcut)  *) 
+(** **** Exercise: 2 stars (smallstep_bool_shortcut)  *)
 (** Suppose we want to add a "short circuit" to the step relation for
     boolean expressions, so that it can recognize when the [then] and
     [else] branches of a conditional are the same value (either
     [ttrue] or [tfalse]) and reduce the whole conditional to this
     value in a single step, even if the guard has not yet been reduced
     to a value. For example, we would like this proposition to be
-    provable: 
+    provable:
          tif
             (tif ttrue ttrue ttrue)
             tfalse
             tfalse
-     ==> 
+     ==>
          tfalse.
 *)
 
@@ -775,7 +815,8 @@ Inductive step : tm -> tm -> Prop :=
   | ST_If : forall t1 t1' t2 t3,
       t1 ==> t1' ->
       tif t1 t2 t3 ==> tif t1' t2 t3
-(* FILL IN HERE *)
+  | ST_ShortCircuit : forall t1 t2,
+      tif t1 t2 t2 ==> t2
 
   where " t '==>' t' " := (step t t').
 
@@ -784,13 +825,13 @@ Definition bool_step_prop4 :=
             (tif ttrue ttrue ttrue)
             tfalse
             tfalse
-     ==> 
+     ==>
          tfalse.
 
-Example bool_step_prop4_holds : 
+Example bool_step_prop4_holds :
   bool_step_prop4.
 Proof.
-  (* FILL IN HERE *) Admitted.
+  constructor. Qed.
 (** [] *)
 
 (** **** Exercise: 3 stars, optional (properties_of_altered_step)  *)
@@ -804,8 +845,15 @@ Proof.
 
       Optional: prove your answer correct in Coq.
 *)
+Theorem step_deterministic :
+  ~ deterministic step.
+Proof.
+  unfold deterministic. unfold not. intros.
+  assert (tif ttrue ttrue ttrue = ttrue).
+  apply H with (tif (tif ttrue ttrue ttrue) ttrue ttrue);
+    repeat constructor. inversion H0.
+Qed.
 
-(* FILL IN HERE *)
 (**
    - Does a strong progress theorem hold? Write yes or no and
      briefly (1 sentence) explain your answer.
@@ -813,14 +861,26 @@ Proof.
      Optional: prove your answer correct in Coq.
 *)
 
-(* FILL IN HERE *)
+Theorem strong_progress : forall t,
+  value t \/ (exists t', t ==> t').
+Proof.
+  intros.
+  induction t;
+  try (left; constructor).
+  right. destruct IHt1.
+  inversion H; subst.
+  exists t2. constructor.
+  exists t3. constructor.
+  destruct H.
+  exists (tif x t2 t3). constructor. assumption.
+Qed.
 (**
    - In general, is there any way we could cause strong progress to
      fail if we took away one or more constructors from the original
      step relation? Write yes or no and briefly (1 sentence) explain
      your answer.
 
-(* FILL IN HERE *)
+remove ST_IfTrue. then (tif ttrue ttrue tfalse) fails strong_progress
 *)
 (** [] *)
 
@@ -832,7 +892,7 @@ End Temp4.
 
 (** Until now, we've been working with the _single-step reduction_
     relation [==>], which formalizes the individual steps of an
-    _abstract machine_ for executing programs.  
+    _abstract machine_ for executing programs.
 
     We can also use this machine to reduce programs to completion --
     to find out what final result they yield.  This can be formalized
@@ -849,7 +909,7 @@ End Temp4.
 
 (** Since we'll want to reuse the idea of multi-step reduction many
     times in this and future chapters, let's take a little extra
-    trouble here and define it generically.  
+    trouble here and define it generically.
 
     Given a relation [R], we define a relation [multi R], called the
     _multi-step closure of [R]_ as follows: *)
@@ -862,7 +922,7 @@ Inductive multi {X:Type} (R: relation X) : relation X :=
                     multi R x z.
 
 (** The effect of this definition is that [multi R] relates two
-    elements [x] and [y] if either 
+    elements [x] and [y] if either
 
        - [x = y], or else
        - there is some sequence [z1], [z2], ..., [zn]
@@ -916,8 +976,8 @@ Proof.
   intros X R x y z G H.
   multi_cases (induction G) Case.
     Case "multi_refl". assumption.
-    Case "multi_step". 
-      apply multi_step with y. assumption. 
+    Case "multi_step".
+      apply multi_step with y. assumption.
       apply IHG. assumption.  Qed.
 
 (** That is, if [t1==>*t2] and [t2==>*t3], then [t1==>*t3]. *)
@@ -929,10 +989,10 @@ Lemma test_multistep_1:
       P
         (P (C 0) (C 3))
         (P (C 2) (C 4))
-   ==>* 
+   ==>*
       C ((0 + 3) + (2 + 4)).
 Proof.
-  apply multi_step with 
+  apply multi_step with
             (P
                 (C (0 + 3))
                 (P (C 2) (C 4))).
@@ -941,9 +1001,9 @@ Proof.
             (P
                 (C (0 + 3))
                 (C (2 + 4))).
-  apply ST_Plus2. apply v_const. 
-  apply ST_PlusConstConst. 
-  apply multi_R. 
+  apply ST_Plus2. apply v_const.
+  apply ST_PlusConstConst.
+  apply multi_R.
   apply ST_PlusConstConst. Qed.
 
 (** Here's an alternate proof that uses [eapply] to avoid explicitly
@@ -957,7 +1017,7 @@ Lemma test_multistep_1':
       C ((0 + 3) + (2 + 4)).
 Proof.
   eapply multi_step. apply ST_Plus1. apply ST_PlusConstConst.
-  eapply multi_step. apply ST_Plus2. apply v_const. 
+  eapply multi_step. apply ST_Plus2. apply v_const.
   apply ST_PlusConstConst.
   eapply multi_step. apply ST_PlusConstConst.
   apply multi_refl.  Qed.
@@ -966,7 +1026,7 @@ Proof.
 Lemma test_multistep_2:
   C 3 ==>* C 3.
 Proof.
-  (* FILL IN HERE *) Admitted.
+  constructor. Qed.
 (** [] *)
 
 (** **** Exercise: 1 star, optional (test_multistep_3)  *)
@@ -975,7 +1035,7 @@ Lemma test_multistep_3:
    ==>*
       P (C 0) (C 3).
 Proof.
-  (* FILL IN HERE *) Admitted.
+  constructor. Qed.
 (** [] *)
 
 (** **** Exercise: 2 stars (test_multistep_4)  *)
@@ -990,7 +1050,11 @@ Lemma test_multistep_4:
         (C 0)
         (C (2 + (0 + 3))).
 Proof.
-  (* FILL IN HERE *) Admitted.
+  econstructor. apply ST_Plus2. constructor.
+  apply ST_Plus2. constructor. constructor.
+  econstructor. apply ST_Plus2. constructor.
+  constructor. constructor.
+Qed.
 (** [] *)
 
 (* ########################################################### *)
@@ -1016,12 +1080,21 @@ Theorem normal_forms_unique:
   deterministic normal_form_of.
 Proof.
   unfold deterministic. unfold normal_form_of.  intros x y1 y2 P1 P2.
-  inversion P1 as [P11 P12]; clear P1. inversion P2 as [P21 P22]; clear P2. 
-  generalize dependent y2. 
+  inversion P1 as [P11 P12]; clear P1. inversion P2 as [P21 P22]; clear P2.
+  generalize dependent y2.
   (* We recommend using this initial setup as-is! *)
-  (* FILL IN HERE *) Admitted.
+  induction P11; intros; unfold step_normal_form in *;
+  unfold normal_form in *. inversion P21.
+  reflexivity. apply ex_falso_quodlibet. apply P12. exists y; assumption.
+  induction P21. apply ex_falso_quodlibet. apply P22. exists y; assumption.
+  assert (y0 = y).
+  eapply step_deterministic; eauto. subst.
+  apply IHP11; assumption.
+Qed.
+
+
 (** [] *)
-  
+
 (** Indeed, something stronger is true for this language (though not
     for all languages): the reduction of _any_ term [t] will
     eventually reach a normal form -- i.e., [normal_form_of] is a
@@ -1045,9 +1118,9 @@ Lemma multistep_congr_1 : forall t1 t1' t2,
      P t1 t2 ==>* P t1' t2.
 Proof.
   intros t1 t1' t2 H. multi_cases (induction H) Case.
-    Case "multi_refl". apply multi_refl. 
-    Case "multi_step". apply multi_step with (P y t2). 
-        apply ST_Plus1. apply H. 
+    Case "multi_refl". apply multi_refl.
+    Case "multi_step". apply multi_step with (P y t2).
+        apply ST_Plus1. apply H.
         apply IHmulti.  Qed.
 
 (** **** Exercise: 2 stars (multistep_congr_2)  *)
@@ -1056,7 +1129,10 @@ Lemma multistep_congr_2 : forall t1 t2 t2',
      t2 ==>* t2' ->
      P t1 t2 ==>* P t1 t2'.
 Proof.
-  (* FILL IN HERE *) Admitted.
+  intros. induction H0. constructor.
+  econstructor. apply ST_Plus2. assumption. eassumption.
+  assumption.
+Qed.
 (** [] *)
 
 (** _Theorem_: The [step] function is normalizing -- i.e., for every
@@ -1071,7 +1147,7 @@ Proof.
       reflexivity and the right-hand side by observing (a) that values
       are normal forms (by [nf_same_as_value]) and (b) that [t] is a
       value (by [v_const]).
-      
+
     - [t = P t1 t2] for some [t1] and [t2].  By the IH, [t1] and
       [t2] have normal forms [t1'] and [t2'].  Recall that normal
       forms are values (by [nf_same_as_value]); we know that [t1' =
@@ -1087,11 +1163,11 @@ Theorem step_normalizing :
 Proof.
   unfold normalizing.
   tm_cases (induction t) Case.
-    Case "C". 
-      exists (C n). 
+    Case "C".
+      exists (C n).
       split.
-      SCase "l". apply multi_refl. 
-      SCase "r". 
+      SCase "l". apply multi_refl.
+      SCase "r".
         (* We can use [rewrite] with "iff" statements, not
            just equalities: *)
         rewrite nf_same_as_value. apply v_const.
@@ -1099,19 +1175,19 @@ Proof.
       inversion IHt1 as [t1' H1]; clear IHt1. inversion IHt2 as [t2' H2]; clear IHt2.
       inversion H1 as [H11 H12]; clear H1. inversion H2 as [H21 H22]; clear H2.
       rewrite nf_same_as_value in H12. rewrite nf_same_as_value in H22.
-      inversion H12 as [n1]. inversion H22 as [n2]. 
-      rewrite <- H in H11. 
+      inversion H12 as [n1]. inversion H22 as [n2].
+      rewrite <- H in H11.
       rewrite <- H0 in H21.
       exists (C (n1 + n2)).
       split.
-        SCase "l". 
+        SCase "l".
           apply multi_trans with (P (C n1) t2).
           apply multistep_congr_1. apply H11.
-          apply multi_trans with 
+          apply multi_trans with
              (P (C n1) (C n2)).
           apply multistep_congr_2. apply v_const. apply H21.
           apply multi_R. apply ST_PlusConstConst.
-        SCase "r". 
+        SCase "r".
           rewrite nf_same_as_value. apply v_const.  Qed.
 
 (* ########################################################### *)
@@ -1128,16 +1204,16 @@ Theorem eval__multistep : forall t n,
   t || n -> t ==>* C n.
 
 (** The key idea behind the proof comes from the following picture:
-       P t1 t2 ==>            (by ST_Plus1) 
-       P t1' t2 ==>           (by ST_Plus1)  
-       P t1'' t2 ==>          (by ST_Plus1) 
-       ...                
+       P t1 t2 ==>            (by ST_Plus1)
+       P t1' t2 ==>           (by ST_Plus1)
+       P t1'' t2 ==>          (by ST_Plus1)
+       ...
        P (C n1) t2 ==>        (by ST_Plus2)
        P (C n1) t2' ==>       (by ST_Plus2)
        P (C n1) t2'' ==>      (by ST_Plus2)
-       ...                
+       ...
        P (C n1) (C n2) ==>    (by ST_PlusConstConst)
-       C (n1 + n2)              
+       C (n1 + n2)
     That is, the multistep reduction of a term of the form [P t1 t2]
     proceeds in three phases:
        - First, we use [ST_Plus1] some number of times to reduce [t1]
@@ -1156,13 +1232,19 @@ Theorem eval__multistep : forall t n,
     includes [==>]. *)
 
 Proof.
-  (* FILL IN HERE *) Admitted.
+  intros. induction H. constructor.
+  apply multi_trans with (P (C n1) t2).
+  apply multistep_congr_1. assumption.
+  apply multi_trans with (P (C n1) (C n2)).
+  apply multistep_congr_2. constructor. assumption.
+  econstructor; constructor.
+Qed.
 (** [] *)
 
 (** **** Exercise: 3 stars, advanced (eval__multistep_inf)  *)
 (** Write a detailed informal version of the proof of [eval__multistep].
 
-(* FILL IN HERE *)
+...
 []
 *)
 (** For the other direction, we need one lemma, which establishes a
@@ -1175,11 +1257,15 @@ Lemma step__eval : forall t t' n,
      t || n.
 Proof.
   intros t t' n Hs. generalize dependent n.
-  (* FILL IN HERE *) Admitted.
+  induction Hs; intros; subst. inversion H. constructor; constructor.
+  inversion H; subst. apply IHHs in H2.
+  constructor; assumption.
+  inversion H0; subst. constructor. assumption. apply IHHs. assumption.
+Qed.
 (** [] *)
 
 (** The fact that small-step reduction implies big-step is now
-    straightforward to prove, once it is stated correctly. 
+    straightforward to prove, once it is stated correctly.
 
     The proof proceeds by induction on the multi-step reduction
     sequence that is buried in the hypothesis [normal_form_of t t']. *)
@@ -1190,7 +1276,14 @@ Proof.
 Theorem multistep__eval : forall t t',
   normal_form_of t t' -> exists n, t' = C n /\ t || n.
 Proof.
-  (* FILL IN HERE *) Admitted.
+  unfold normal_form_of. unfold step_normal_form. intros.
+  destruct H. induction H.
+  apply nf_is_value in H0. inversion H0; subst. exists n.
+  split. reflexivity. constructor.
+  apply IHmulti in H0. destruct H0. destruct H0.
+  exists x0. split. assumption. eapply step__eval. eassumption.
+  assumption.
+Qed.
 (** [] *)
 
 (* ########################################################### *)
@@ -1200,7 +1293,7 @@ Proof.
 (** Remember that we also defined big-step evaluation of [tm]s as a
     function [evalF].  Prove that it is equivalent to the existing
     semantics.
- 
+
     Hint: we just proved that [eval] and [multistep] are
     equivalent, so logically it doesn't matter which you choose.
     One will be easier than the other, though!  *)
@@ -1208,7 +1301,12 @@ Proof.
 Theorem evalF_eval : forall t n,
   evalF t = n <-> t || n.
 Proof.
-  (* FILL IN HERE *) Admitted.
+  split; intros; generalize dependent n;
+  induction t; intros; simpl in *; subst.
+  constructor. constructor. apply IHt1. reflexivity. apply IHt2. reflexivity.
+  inversion H. reflexivity.
+  inversion H. apply IHt1 in H2. apply IHt2 in H4. subst. reflexivity.
+Qed.
 (** [] *)
 
 (** **** Exercise: 4 stars (combined_properties)  *)
@@ -1243,7 +1341,7 @@ Inductive step : tm -> tm -> Prop :=
       t1 ==> t1' ->
       P t1 t2 ==> P t1' t2
   | ST_Plus2 : forall v1 t2 t2',
-      value v1 ->     
+      value v1 ->
       t2 ==> t2' ->
       P v1 t2 ==> P v1 t2'
   | ST_IfTrue : forall t1 t2,
@@ -1271,7 +1369,31 @@ Tactic Notation "step_cases" tactic(first) ident(c) :=
 
     Prove or disprove these two properties for the combined language. *)
 
-(* FILL IN HERE *)
+Theorem step_deterministic:
+  deterministic step.
+Proof.
+  unfold deterministic. intros.
+  generalize dependent y2.
+  induction H; intros; subst.
+  inversion H0. reflexivity. inversion H3. inversion H4.
+  inversion H0; subst; try (solve by inversion).
+  apply IHstep in H4. subst. reflexivity.
+  inversion H3; subst; try (solve by inversion).
+  inversion H1; subst; try (solve by inversion).
+  inversion H; subst; try (solve by inversion).
+  apply IHstep in H6. subst. reflexivity.
+  inversion H0; subst. reflexivity. inversion H4.
+  inversion H0; subst. reflexivity. inversion H4.
+  inversion H0; subst; try (solve by inversion).
+  apply IHstep in H5. subst. reflexivity.
+Qed.
+
+Theorem weak_progress : exists t,
+  ~ value t /\ ~ (exists t', t ==> t').
+Proof.
+  exists (P ttrue ttrue). split; unfold not; intros.
+  inversion H. inversion H. inversion H0; try (solve by inversion).
+Qed.
 (** [] *)
 
 End Combined.
@@ -1300,7 +1422,7 @@ Inductive aval : aexp -> Prop :=
 Reserved Notation " t '/' st '==>a' t' " (at level 40, st at level 39).
 
 Inductive astep : state -> aexp -> aexp -> Prop :=
-  | AS_Id : forall st i, 
+  | AS_Id : forall st i,
       AId i / st ==>a ANum (st i)
   | AS_Plus : forall st n1 n2,
       APlus (ANum n1) (ANum n2) / st ==>a ANum (n1 + n2)
@@ -1336,17 +1458,17 @@ Inductive astep : state -> aexp -> aexp -> Prop :=
 
   Inductive bstep : state -> bexp -> bexp -> Prop :=
   | BS_Eq : forall st n1 n2,
-      (BEq (ANum n1) (ANum n2)) / st ==>b 
+      (BEq (ANum n1) (ANum n2)) / st ==>b
       (if (beq_nat n1 n2) then BTrue else BFalse)
   | BS_Eq1 : forall st a1 a1' a2,
       a1 / st ==>a a1' ->
       (BEq a1 a2) / st ==>b (BEq a1' a2)
   | BS_Eq2 : forall st v1 a2 a2',
-      aval v1 -> 
+      aval v1 ->
       a2 / st ==>a a2' ->
       (BEq v1 a2) / st ==>b (BEq v1 a2')
   | BS_LtEq : forall st n1 n2,
-      (BLe (ANum n1) (ANum n2)) / st ==>b 
+      (BLe (ANum n1) (ANum n2)) / st ==>b
                (if (ble_nat n1 n2) then BTrue else BFalse)
   | BS_LtEq1 : forall st a1 a1' a2,
       a1 / st ==>a a1' ->
@@ -1381,7 +1503,7 @@ Inductive astep : state -> aexp -> aexp -> Prop :=
     small tricks to make it work:
 
        - We use [SKIP] as a "command value" -- i.e., a command that
-         has reached a normal form.  
+         has reached a normal form.
 
             - An assignment command reduces to [SKIP] (and an updated
               state).
@@ -1399,14 +1521,14 @@ Inductive astep : state -> aexp -> aexp -> Prop :=
    command needs to be saved somewhere while a single copy of the loop
    body is being evaluated.) *)
 
-Reserved Notation " t '/' st '==>' t' '/' st' " 
+Reserved Notation " t '/' st '==>' t' '/' st' "
                   (at level 40, st at level 39, t' at level 39).
 
 Inductive cstep : (com * state) -> (com * state) -> Prop :=
   | CS_AssStep : forall st i a a',
       a / st ==>a a' ->
-      (i ::= a) / st ==> (i ::= a') / st 
-  | CS_Ass : forall st i n, 
+      (i ::= a) / st ==> (i ::= a') / st
+  | CS_Ass : forall st i n,
       (i ::= (ANum n)) / st ==> SKIP / (update st i n)
   | CS_SeqStep : forall st c1 c1' st' c2,
       c1 / st ==> c1' / st' ->
@@ -1453,25 +1575,25 @@ Tactic Notation "com_cases" tactic(first) ident(c) :=
   [ Case_aux c "SKIP" | Case_aux c "::=" | Case_aux c ";"
   | Case_aux c "IFB" | Case_aux c "WHILE" | Case_aux c "PAR" ].
 
-Notation "'SKIP'" := 
+Notation "'SKIP'" :=
   CSkip.
-Notation "x '::=' a" := 
+Notation "x '::=' a" :=
   (CAss x a) (at level 60).
-Notation "c1 ;; c2" := 
+Notation "c1 ;; c2" :=
   (CSeq c1 c2) (at level 80, right associativity).
-Notation "'WHILE' b 'DO' c 'END'" := 
+Notation "'WHILE' b 'DO' c 'END'" :=
   (CWhile b c) (at level 80, right associativity).
-Notation "'IFB' b 'THEN' c1 'ELSE' c2 'FI'" := 
+Notation "'IFB' b 'THEN' c1 'ELSE' c2 'FI'" :=
   (CIf b c1 c2) (at level 80, right associativity).
-Notation "'PAR' c1 'WITH' c2 'END'" := 
+Notation "'PAR' c1 'WITH' c2 'END'" :=
   (CPar c1 c2) (at level 80, right associativity).
 
 Inductive cstep : (com * state)  -> (com * state) -> Prop :=
     (* Old part *)
   | CS_AssStep : forall st i a a',
-      a / st ==>a a' -> 
+      a / st ==>a a' ->
       (i ::= a) / st ==> (i ::= a') / st
-  | CS_Ass : forall st i n, 
+  | CS_Ass : forall st i n,
       (i ::= (ANum n)) / st ==> SKIP / (update st i n)
   | CS_SeqStep : forall st c1 c1' st' c2,
       c1 / st ==> c1' / st' ->
@@ -1483,14 +1605,14 @@ Inductive cstep : (com * state)  -> (com * state) -> Prop :=
   | CS_IfFalse : forall st c1 c2,
       (IFB BFalse THEN c1 ELSE c2 FI) / st ==> c2 / st
   | CS_IfStep : forall st b b' c1 c2,
-      b /st ==>b b' -> 
+      b /st ==>b b' ->
       (IFB b THEN c1 ELSE c2 FI) / st ==> (IFB b' THEN c1 ELSE c2 FI) / st
   | CS_While : forall st b c1,
-      (WHILE b DO c1 END) / st ==> 
+      (WHILE b DO c1 END) / st ==>
                (IFB b THEN (c1;; (WHILE b DO c1 END)) ELSE SKIP FI) / st
     (* New part: *)
   | CS_Par1 : forall st c1 c1' c2 st',
-      c1 / st ==> c1' / st' -> 
+      c1 / st ==> c1' / st' ->
       (PAR c1 WITH c2 END) / st ==> (PAR c1' WITH c2 END) / st'
   | CS_Par2 : forall st c1 c2 c2' st',
       c2 / st ==> c2' / st' ->
@@ -1500,11 +1622,11 @@ Inductive cstep : (com * state)  -> (com * state) -> Prop :=
   where " t '/' st '==>' t' '/' st' " := (cstep (t,st) (t',st')).
 
 
-Definition cmultistep := multi cstep. 
+Definition cmultistep := multi cstep.
 
-Notation " t '/' st '==>*' t' '/' st' " := 
-   (multi cstep  (t,st) (t',st')) 
-   (at level 40, st at level 39, t' at level 39).  
+Notation " t '/' st '==>*' t' '/' st' " :=
+   (multi cstep  (t,st) (t',st'))
+   (at level 40, st at level 39, t' at level 39).
 
 
 
@@ -1532,16 +1654,16 @@ Example par_loop_example_0:
 Proof.
   eapply ex_intro. split.
   unfold par_loop.
-  eapply multi_step. apply CS_Par1. 
+  eapply multi_step. apply CS_Par1.
     apply CS_Ass.
   eapply multi_step. apply CS_Par2. apply CS_While.
-  eapply multi_step. apply CS_Par2. apply CS_IfStep. 
+  eapply multi_step. apply CS_Par2. apply CS_IfStep.
     apply BS_Eq1. apply AS_Id.
-  eapply multi_step. apply CS_Par2. apply CS_IfStep. 
-    apply BS_Eq. simpl. 
-  eapply multi_step. apply CS_Par2. apply CS_IfFalse. 
-  eapply multi_step. apply CS_ParDone. 
-  eapply multi_refl. 
+  eapply multi_step. apply CS_Par2. apply CS_IfStep.
+    apply BS_Eq. simpl.
+  eapply multi_step. apply CS_Par2. apply CS_IfFalse.
+  eapply multi_step. apply CS_ParDone.
+  eapply multi_refl.
   reflexivity. Qed.
 
 (** It can also terminate with [X] set to [2]: *)
@@ -1553,43 +1675,43 @@ Example par_loop_example_2:
 Proof.
   eapply ex_intro. split.
   eapply multi_step. apply CS_Par2. apply CS_While.
-  eapply multi_step. apply CS_Par2. apply CS_IfStep. 
+  eapply multi_step. apply CS_Par2. apply CS_IfStep.
     apply BS_Eq1. apply AS_Id.
-  eapply multi_step. apply CS_Par2. apply CS_IfStep. 
-    apply BS_Eq. simpl. 
-  eapply multi_step. apply CS_Par2. apply CS_IfTrue. 
+  eapply multi_step. apply CS_Par2. apply CS_IfStep.
+    apply BS_Eq. simpl.
+  eapply multi_step. apply CS_Par2. apply CS_IfTrue.
   eapply multi_step. apply CS_Par2. apply CS_SeqStep.
     apply CS_AssStep. apply AS_Plus1. apply AS_Id.
   eapply multi_step. apply CS_Par2. apply CS_SeqStep.
-    apply CS_AssStep. apply AS_Plus.  
+    apply CS_AssStep. apply AS_Plus.
   eapply multi_step. apply CS_Par2. apply CS_SeqStep.
     apply CS_Ass.
   eapply multi_step. apply CS_Par2. apply CS_SeqFinish.
 
   eapply multi_step. apply CS_Par2. apply CS_While.
-  eapply multi_step. apply CS_Par2. apply CS_IfStep. 
+  eapply multi_step. apply CS_Par2. apply CS_IfStep.
     apply BS_Eq1. apply AS_Id.
-  eapply multi_step. apply CS_Par2. apply CS_IfStep. 
-    apply BS_Eq. simpl. 
-  eapply multi_step. apply CS_Par2. apply CS_IfTrue. 
+  eapply multi_step. apply CS_Par2. apply CS_IfStep.
+    apply BS_Eq. simpl.
+  eapply multi_step. apply CS_Par2. apply CS_IfTrue.
   eapply multi_step. apply CS_Par2. apply CS_SeqStep.
     apply CS_AssStep. apply AS_Plus1. apply AS_Id.
   eapply multi_step. apply CS_Par2. apply CS_SeqStep.
-    apply CS_AssStep. apply AS_Plus.  
+    apply CS_AssStep. apply AS_Plus.
   eapply multi_step. apply CS_Par2. apply CS_SeqStep.
     apply CS_Ass.
 
   eapply multi_step. apply CS_Par1. apply CS_Ass.
   eapply multi_step. apply CS_Par2. apply CS_SeqFinish.
   eapply multi_step. apply CS_Par2. apply CS_While.
-  eapply multi_step. apply CS_Par2. apply CS_IfStep. 
+  eapply multi_step. apply CS_Par2. apply CS_IfStep.
     apply BS_Eq1. apply AS_Id.
-  eapply multi_step. apply CS_Par2. apply CS_IfStep. 
-    apply BS_Eq. simpl. 
-  eapply multi_step. apply CS_Par2. apply CS_IfFalse. 
-  eapply multi_step. apply CS_ParDone. 
-  eapply multi_refl. 
-  reflexivity. Qed. 
+  eapply multi_step. apply CS_Par2. apply CS_IfStep.
+    apply BS_Eq. simpl.
+  eapply multi_step. apply CS_Par2. apply CS_IfFalse.
+  eapply multi_step. apply CS_ParDone.
+  eapply multi_refl.
+  reflexivity. Qed.
 
 (** More generally... *)
 
@@ -1598,7 +1720,22 @@ Lemma par_body_n__Sn : forall n st,
   st X = n /\ st Y = 0 ->
   par_loop / st ==>* par_loop / (update st X (S n)).
 Proof.
-  (* FILL IN HERE *) Admitted.
+  intros. destruct H.
+  eapply multi_step. apply CS_Par2. apply CS_While.
+  eapply multi_step. apply CS_Par2. apply CS_IfStep.
+  apply BS_Eq1. apply AS_Id.
+  eapply multi_step. apply CS_Par2. apply CS_IfStep.
+  apply BS_Eq. rewrite H0. simpl.
+  eapply multi_step. apply CS_Par2. apply CS_IfTrue.
+  eapply multi_step. apply CS_Par2. apply CS_SeqStep.
+  apply CS_AssStep. apply AS_Plus1. apply AS_Id.
+  eapply multi_step. apply CS_Par2. apply CS_SeqStep.
+  rewrite H. apply CS_AssStep. apply AS_Plus.
+  eapply multi_step. apply CS_Par2. apply CS_SeqStep.
+  apply CS_Ass.
+  eapply multi_step. apply CS_Par2. apply CS_SeqFinish.
+  assert (n + 1 = S n) by omega. rewrite H1. apply multi_refl.
+Qed.
 (** [] *)
 
 (** **** Exercise: 3 stars, optional  *)
@@ -1607,7 +1744,14 @@ Lemma par_body_n : forall n st,
   exists st',
     par_loop / st ==>*  par_loop / st' /\ st' X = n /\ st' Y = 0.
 Proof.
-  (* FILL IN HERE *) Admitted.
+  intros n. induction n; intros.
+  exists st. split. constructor. assumption.
+  apply IHn in H. destruct H. destruct H. exists (update x X (S n)).
+  split. eapply multi_trans. apply H. apply par_body_n__Sn. assumption.
+  split. rewrite update_eq. reflexivity.
+  rewrite update_neq. destruct H0. assumption. unfold not. intros.
+  inversion H1.
+Qed.
 (** [] *)
 
 (** ... the above loop can exit with [X] having any value
@@ -1618,14 +1762,14 @@ Theorem par_loop_any_X:
     par_loop / empty_state ==>*  SKIP / st'
     /\ st' X = n.
 Proof.
-  intros n. 
-  destruct (par_body_n n empty_state). 
+  intros n.
+  destruct (par_body_n n empty_state).
     split; unfold update; reflexivity.
 
   rename x into st.
-  inversion H as [H' [HX HY]]; clear H. 
+  inversion H as [H' [HX HY]]; clear H.
   exists (update st Y 1). split.
-  eapply multi_trans with (par_loop,st). apply H'. 
+  eapply multi_trans with (par_loop,st). apply H'.
   eapply multi_step. apply CS_Par1. apply CS_Ass.
   eapply multi_step. apply CS_Par2. apply CS_While.
   eapply multi_step. apply CS_Par2. apply CS_IfStep.
@@ -1636,7 +1780,7 @@ Proof.
   eapply multi_step. apply CS_ParDone.
   apply multi_refl.
 
-  rewrite update_neq. assumption. intro X; inversion X. 
+  rewrite update_neq. assumption. intro X; inversion X.
 Qed.
 
 End CImp.
@@ -1662,7 +1806,7 @@ Inductive stack_step : state -> prog * stack -> prog * stack -> Prop :=
   | SS_Mult : forall st stk n m p',
     stack_step st (SMult :: p', n::m::stk)  (p', (m*n)::stk).
 
-Theorem stack_step_deterministic : forall st, 
+Theorem stack_step_deterministic : forall st,
   deterministic (stack_step st).
 Proof.
   unfold deterministic. intros st x y1 y2 H1 H2.
@@ -1672,22 +1816,46 @@ Qed.
 Definition stack_multistep st := multi (stack_step st).
 
 (** **** Exercise: 3 stars, advanced (compiler_is_correct)  *)
-(** Remember the definition of [compile] for [aexp] given in the 
+(** Remember the definition of [compile] for [aexp] given in the
     [Imp] chapter. We want now to prove [compile] correct with respect
     to the stack machine.
 
-    State what it means for the compiler to be correct according to 
+    State what it means for the compiler to be correct according to
     the stack machine small step semantics and then prove it. *)
 
-Definition compiler_is_correct_statement : Prop := 
-(* FILL IN HERE *) admit.
+Definition compiler_is_correct_statement : Prop :=
+  forall e st stk p, stack_multistep st ((s_compile e) ++ p, stk) (p, aeval st e :: stk).
 
 
 Theorem compiler_is_correct : compiler_is_correct_statement.
 Proof.
-(* FILL IN HERE *) Admitted.
+  unfold compiler_is_correct_statement. unfold stack_multistep.
+  intros e. induction e; intros; simpl;
+  try (eapply multi_step; constructor; apply multi_refl).
+  Case "Plus".
+  apply multi_trans with (s_compile e2 ++ [SPlus] ++ p, aeval st e1 :: stk).
+  rewrite <- app_assoc. rewrite <- (app_assoc (s_compile e2) [SPlus] p).
+  apply IHe1.
+  apply multi_trans with ([SPlus] ++ p, aeval st e2 :: aeval st e1 :: stk).
+  apply IHe2. apply multi_trans with (p, aeval st e1 + aeval st e2 :: stk).
+  eapply multi_step. constructor. simpl. apply multi_refl.
+  rewrite plus_comm. apply multi_refl.
+  Case "Minus".
+  apply multi_trans with (s_compile e2 ++ [SMinus] ++ p, aeval st e1 :: stk).
+  rewrite <- app_assoc. rewrite <- (app_assoc (s_compile e2) [SMinus] p).
+  apply IHe1.
+  apply multi_trans with ([SMinus] ++ p, aeval st e2 :: aeval st e1 :: stk).
+  apply IHe2. apply multi_trans with (p, aeval st e1 - aeval st e2 :: stk).
+  eapply multi_step. constructor. simpl. apply multi_refl. apply multi_refl.
+  Case "Multi".
+  apply multi_trans with (s_compile e2 ++ [SMult] ++ p, aeval st e1 :: stk).
+  rewrite <- app_assoc. rewrite <- (app_assoc (s_compile e2) [SMult] p).
+  apply IHe1.
+  apply multi_trans with ([SMult] ++ p, aeval st e2 :: aeval st e1 :: stk).
+  apply IHe2. apply multi_trans with (p, aeval st e1 * aeval st e2 :: stk).
+  eapply multi_step. constructor. simpl. apply multi_refl.
+  rewrite mult_comm. apply multi_refl.
+Qed.
 (** [] *)
 
 (** $Date: 2014-12-31 15:16:58 -0500 (Wed, 31 Dec 2014) $ *)
-
-
